src/opt/Reorder.v
@@ -33,30 +33,51 @@ Inductive reorder: forall (i1 i2:Instr.t), Prop :=
     (DISJOINT: RegSet.disjoint (Instr.regs_of (Instr.load r1 l1 Ordering.relaxed))
                                (Instr.regs_of (Instr.store l2 v2 Ordering.relaxed))):
     reorder (Instr.load r1 l1 Ordering.relaxed) (Instr.store l2 v2 Ordering.relaxed)
+| reorder_store_store
+    l1 v1 ord1
+    l2 v2
+    (LOC: l1 <> l2)
+    (DISJOINT: RegSet.disjoint (Instr.regs_of (Instr.store l1 v1 ord1))
+                               (Instr.regs_of (Instr.store l2 v2 Ordering.relaxed))):
+    reorder (Instr.store l1 v1 ord1) (Instr.store l2 v2 Ordering.relaxed)
 .
 
 Inductive sim_reorder (i1:Instr.t) (l2:Loc.t) (v2:Value.t) (o2:Ordering.t):
   forall (th_src:Thread.t lang) (mem_k_src:Memory.t)
     (th_tgt:Thread.t lang) (mem_k_tgt:Memory.t), Prop :=
-| sim_reorder_phase0
+| sim_reorder_begin
     rs
     commit_src commit_tgt
-    promise
+    promise_src promise_tgt
     mem_k_src mem_k_tgt
-    (COMMIT: Commit.le commit_src commit_tgt):
+    (COMMIT: Commit.le commit_src commit_tgt)
+    (PROMISE: MemInv.sem Memory.bot promise_src promise_tgt):
     sim_reorder
       i1 l2 v2 o2
-      (Thread.mk lang (State.mk rs [Stmt.instr Instr.nop; Stmt.instr i1; Stmt.instr (Instr.store l2 v2 o2)]) commit_src promise)
+      (Thread.mk lang (State.mk rs [Stmt.instr Instr.nop; Stmt.instr i1; Stmt.instr (Instr.store l2 v2 o2)]) commit_src promise_src)
       mem_k_src
-      (Thread.mk lang (State.mk rs [Stmt.instr (Instr.store l2 v2 o2); Stmt.instr i1]) commit_tgt promise)
+      (Thread.mk lang (State.mk rs [Stmt.instr (Instr.store l2 v2 o2); Stmt.instr i1]) commit_tgt promise_tgt)
       mem_k_tgt
-| sim_reorder_phase1
+| sim_reorder_end
+    rs
+    commit_src commit_tgt
+    promise_src promise_tgt
+    mem_k_src mem_k_tgt
+    (COMMIT: Commit.le commit_src commit_tgt)
+    (PROMISE: MemInv.sem Memory.bot promise_src promise_tgt):
+    sim_reorder
+      i1 l2 v2 o2
+      (Thread.mk lang (State.mk rs []) commit_src promise_src)
+      mem_k_src
+      (Thread.mk lang (State.mk rs []) commit_tgt promise_tgt)
+      mem_k_tgt
+| sim_reorder_intermediate
     rs
     commit_src commit_tgt commit_imm
     promise_src promise_tgt
     mem_k_src mem_k_tgt
     from to released
-    (COMMIT1: Commit.write commit_src l2 to released Ordering.relaxed commit_imm)
+    (COMMIT1: Commit.write commit_src l2 to released o2 commit_imm)
     (COMMIT2: Commit.le commit_imm commit_tgt)
     (LT: Time.lt from to)
     (PROMISE: MemInv.sem (Memory.singleton l2 (Message.mk (RegFile.eval_value rs v2) released) LT) promise_src promise_tgt):
@@ -65,18 +86,6 @@ Inductive sim_reorder (i1:Instr.t) (l2:Loc.t) (v2:Value.t) (o2:Ordering.t):
       (Thread.mk lang (State.mk rs [Stmt.instr i1; Stmt.instr (Instr.store l2 v2 o2)]) commit_src promise_src)
       mem_k_src
       (Thread.mk lang (State.mk rs [Stmt.instr i1]) commit_tgt promise_tgt)
-      mem_k_tgt
-| sim_reorder_phase2
-    rs
-    commit_src commit_tgt
-    promise
-    mem_k_src mem_k_tgt
-    (COMMIT: Commit.le commit_src commit_tgt):
-    sim_reorder
-      i1 l2 v2 o2
-      (Thread.mk lang (State.mk rs []) commit_src promise)
-      mem_k_src
-      (Thread.mk lang (State.mk rs []) commit_tgt promise)
       mem_k_tgt
 .
 
@@ -95,14 +104,16 @@ Proof.
     + i. eexists. splits; try reflexivity; eauto.
       inv WF_SRC0. inv WF_TGT. econs; ss. eapply Commit.future_wf; eauto.
     + i. eexists. splits; try reflexivity; eauto.
+      inv WF_SRC0. inv WF_TGT. econs; ss. eapply Commit.future_wf; eauto.
+    + i. eexists. splits; try reflexivity; eauto.
       inv WF_SRC0. inv WF_TGT. econs; ss.
       * eapply Commit.future_wf; eauto.
       * rewrite <- PROMISE0. inv PROMISE. apply Memory.le_join_l. memtac.
-    + i. eexists. splits; try reflexivity; eauto.
-      inv WF_SRC0. inv WF_TGT. econs; ss. eapply Commit.future_wf; eauto.
   - i. inv PR; ss.
-    + eexists _, _. splits; eauto.
-    + inv REORDER.
+    { eexists _, _. splits; eauto. }
+    { eexists _, _. splits; eauto. }
+    inv REORDER.
+    + (* load *)
       exploit MemInv.confirm_src; try apply MEMORY; eauto.
       { econs.
         - rewrite Memory.join_comm, Memory.bot_join. eauto.
@@ -118,15 +129,16 @@ Proof.
       { apply WF_SRC. }
       i. des.
       exploit (@CommitFacts.write_min_spec l2); try apply MEMORY_SRC; eauto.
-      { instantiate (1 := Ordering.relaxed). ss. }
       { eapply Snapshot.le_on_writable; eauto. apply COMMIT1. }
-      { ss. inv COMMIT1. etransitivity; [apply MONOTONE|apply RELEASED]. }
+      { instantiate (1 := Ordering.relaxed).
+        ss. inv COMMIT1. etransitivity; [apply MONOTONE|apply RELEASED].
+      }
       { inv MEMORY_SRC. exploit WF0; eauto. }
       i. des. simpl in WRITE.
       eexists _, _. splits.
       * econs 2; [|econs 2; [|econs 1]].
         { econs. s. instantiate (1 := (_, _)).
-          econs 1; s; eauto.
+          econs 2; s; eauto.
           - econs. econs.
           - inv CONFIRM. rewrite Memory.join_comm, Memory.bot_join.
             match goal with
@@ -134,7 +146,7 @@ Proof.
             end.
             apply Memory.singleton_get_inv in X. des. congruence.
         }
-        { econs. s. econs 2; s; eauto.
+        { econs. s. econs 3; s; eauto.
           - econs. econs.
           - econs 1; ss.
             erewrite RegFile.eq_except_value; eauto.
@@ -142,11 +154,94 @@ Proof.
         }
       * eauto.
       * s. eauto.
-    + eexists _, _. splits; eauto.
+    + (* store *)
+      admit.
   - i. inv STEP_TGT; [|inv STATE; inv INSTR; inv PR; inv REORDER].
-    inv STEP.
-    + (* read, phase 2 *)
-      inv STATE. destruct x2. ss. subst. inv INSTR. inv REORDER. inv PR.
+    inv PR; ss.
+    { (* phase begin *)
+      inv STEP; try (inv STATE; inv INSTR); ss.
+      { exploit MemInv.promise; try apply MEMORY; eauto.
+        { apply WF_SRC. }
+        { apply WF_TGT. }
+        { apply MemInv.sem_bot. }
+        s. i. des. apply MemInv.sem_bot_inv in INV2. subst.
+        exploit Memory.promise_future; try apply PROMISE_SRC; eauto.
+        { apply WF_SRC. }
+        i. des.
+        eexists _, _, _, _. splits; eauto.
+        - instantiate (1 := Thread.mk _ _ _ _). econs 1. econs 1; s; eauto.
+          inv WF_TGT. eapply Commit.future_wf; eauto.
+          etransitivity; eauto. inv MEMORY. apply Memory.splits_future. auto.
+        - right. apply CIH. econs 1. auto.
+      }
+      inv MEMORY0.
+      - exploit MemInv.confirm; try apply MEMORY; eauto.
+        { apply WF_SRC. }
+        { apply WF_TGT. }
+        { apply MemInv.sem_bot. }
+        s. i. des.
+        eexists _, _, _, _. splits; eauto.
+        + econs 1. s. econs 6; s.
+          * econs. econs.
+          * reflexivity.
+          * apply WF_SRC.
+        + inv CONFIRM; ss. right. apply CIH. econs 3; eauto.
+          * eapply CommitFacts.write_mon; eauto.
+          * reflexivity.
+          * econs. memtac.
+      - exploit MemInv.add; try apply MEMORY; eauto.
+        { apply WF_SRC. }
+        { apply WF_TGT. }
+        { apply MemInv.sem_bot. }
+        s. i. des. rewrite Memory.join_comm, Memory.bot_join in INV2.
+        exploit Memory.promise_future; try apply PROMISE_SRC; eauto.
+        { apply WF_SRC. }
+        i. des.
+        eexists _, _, _, _. splits.
+        + econs 2; [|econs 1].
+          econs 1. s. econs 6; s.
+          * econs. econs.
+          * reflexivity.
+          * apply WF_SRC.
+        + econs 1. econs 1; eauto.
+          inv WF_TGT. eapply Commit.future_wf; eauto.
+          etransitivity; eauto. inv MEMORY. apply Memory.splits_future. auto.
+        + auto.
+        + ss. right. apply CIH. econs 3; eauto. reflexivity.
+    }
+    { (* phase end *)
+      inv STEP; try (inv STATE; inv INSTR); ss.
+      exploit MemInv.promise; try apply MEMORY; eauto.
+      { apply WF_SRC. }
+      { apply WF_TGT. }
+      { apply MemInv.sem_bot. }
+      s. i. des. apply MemInv.sem_bot_inv in INV2. subst.
+      exploit Memory.promise_future; try apply PROMISE_SRC; eauto.
+      { apply WF_SRC. }
+      i. des.
+      eexists _, _, _, _. splits; eauto.
+      - instantiate (1 := Thread.mk _ _ _ _). econs 1. econs 1; s; eauto.
+        inv WF_TGT. eapply Commit.future_wf; eauto.
+        etransitivity; eauto. inv MEMORY. apply Memory.splits_future. auto.
+      - right. apply CIH. econs 2. auto.
+    }
+    (* phase intermediate *)
+    inv STEP; try by inv REORDER; inv STATE; inv INSTR.
+    { exploit MemInv.promise; try apply MEMORY; eauto.
+        { apply WF_SRC. }
+        { apply WF_TGT. }
+        s. i. des.
+        exploit Memory.promise_future; try apply PROMISE_SRC; eauto.
+        { apply WF_SRC. }
+        i. des.
+        eexists _, _, _, _. splits; eauto.
+        - instantiate (1 := Thread.mk _ _ _ _). econs 1.
+          econs 1; s; try reflexivity; eauto.
+          inv WF_SRC. eapply Commit.future_wf; eauto.
+        - right. apply CIH. econs 3; eauto. etransitivity; eauto.
+    }
+    + (* load *)
+      inv REORDER; inv STATE; inv INSTR.
       exploit MemInv.confirm_src; try apply MEMORY; eauto.
       { econs.
         - rewrite Memory.join_comm, Memory.bot_join. eauto.
@@ -165,14 +260,15 @@ Proof.
       { apply WF_SRC. }
       i. des.
       exploit CommitFacts.write_min_spec; try apply MEMORY_SRC; eauto.
-      { instantiate (1 := Ordering.relaxed). ss. }
       { eapply Snapshot.le_on_writable; eauto. apply COMMIT1. }
-      { ss. inv COMMIT1. etransitivity; [apply MONOTONE|apply RELEASED]. }
+      { instantiate (1 := Ordering.relaxed).
+        ss. inv COMMIT1. etransitivity; [apply MONOTONE|apply RELEASED].
+      }
       { inv MEMORY_SRC. exploit WF0; eauto. }
       i. des.
       eexists _, _, _, _. splits.
       { econs 2; [|econs 1].
-        econs 1. s. econs 1; s; eauto.
+        econs 1. s. econs 2; s; eauto.
         - econs. econs.
         - inv CONFIRM.
           match goal with
@@ -181,13 +277,13 @@ Proof.
           apply Memory.join_get in X; ss. des; [congruence|].
           apply Memory.singleton_get_inv in X. des. subst. congruence.
       }
-      { econs 1. s. econs 2; s; eauto.
+      { econs 1. s. econs 3; s; eauto.
         - econs. econs.
         - econs 1; ss. erewrite RegFile.eq_except_value; eauto.
           apply RegFile.eq_except_singleton.
       }
       { auto. }
-      { right. apply CIH. econs 3.
+      { right. apply CIH. econs 2.
         exploit CommitFacts.write_min_min; try apply COMMIT1; eauto. i.
         exploit CommitFacts.read_min_min; try apply COMMIT; eauto. i.
         inv x4. inv x5. inv CURRENT1. inv CURRENT2. ss. econs; s.
@@ -202,92 +298,57 @@ Proof.
           + etransitivity; [|apply Snapshot.join_r].
             etransitivity; [|apply COMMIT2]. apply COMMIT1.
       }
-    + (* write, phase 1 *)
-      inv STATE. destruct x2. ss. subst. inv INSTR. inv REORDER. inv PR.
-      inv MEMORY0.
-      * exploit MemInv.confirm; try apply MEMORY; eauto.
-        { apply WF_SRC. }
-        { apply WF_TGT. }
-        { apply MemInv.sem_bot. }
-        s. i. des.
-        eexists _, _, _, _. splits; eauto.
-        { econs 1. s. econs 5; s.
-          - econs. econs.
-          - reflexivity.
-          - apply WF_SRC.
-        }
-        { inv CONFIRM; ss. right. apply CIH. econs 2; eauto.
-          - eauto. eapply CommitFacts.write_mon; eauto.
-          - reflexivity.
-          - econs. memtac.
-        }
-      * exploit MemInv.add; try apply MEMORY; eauto.
-        { apply WF_SRC. }
-        { apply WF_TGT. }
-        { apply MemInv.sem_bot. }
-        s. i. des. rewrite Memory.join_comm, Memory.bot_join in INV2.
-        exploit Memory.promise_future; try apply PROMISE_SRC; eauto.
-        { apply WF_SRC. }
-        i. des.
-        eexists _, _, _, _. splits.
-        { econs 2; [|econs 1].
-          econs 1. s. econs 5; s.
-          - econs. econs.
-          - reflexivity.
-          - apply WF_SRC.
-        }
-        { econs 1. econs 6; eauto.
-          inv WF_TGT. eapply Commit.future_wf; eauto.
-          etransitivity; eauto. inv MEMORY. apply Memory.splits_future. auto.
-        }
-        { auto. }
-        ss. right. apply CIH. econs 2; eauto. reflexivity.
-    + inv STATE; destruct x2; ss; subst; try inv INSTR; inv PR; inv REORDER.
-    + inv STATE; destruct x2; ss; subst; try inv INSTR; inv PR; inv REORDER.
-    + inv STATE; destruct x2; ss; subst; try inv INSTR; inv PR; inv REORDER.
-    + inv PR; ss.
-      * exploit MemInv.promise; try apply MEMORY; eauto.
-        { apply WF_SRC. }
-        { apply WF_TGT. }
-        { apply MemInv.sem_bot. }
-        s. i. des. apply MemInv.sem_bot_inv in INV2. subst.
-        exploit Memory.promise_future; try apply PROMISE_SRC; eauto.
-        { apply WF_SRC. }
-        i. des.
-        eexists _, _, _, _. splits; eauto.
-        { instantiate (1 := Thread.mk _ _ _ _). econs 1. econs 6; s; eauto.
-          inv WF_TGT. eapply Commit.future_wf; eauto.
-          etransitivity; eauto. inv MEMORY. apply Memory.splits_future. auto.
-        }
-        { right. apply CIH. econs 1. auto. }
-      * exploit MemInv.promise; try apply MEMORY; eauto.
-        { apply WF_SRC. }
-        { apply WF_TGT. }
-        s. i. des.
-        exploit Memory.promise_future; try apply PROMISE_SRC; eauto.
-        { apply WF_SRC. }
-        i. des.
-        eexists _, _, _, _. splits; eauto.
-        { instantiate (1 := Thread.mk _ _ _ _). econs 1.
-          econs 6; s; try reflexivity; eauto.
-          inv WF_SRC. eapply Commit.future_wf; eauto.
-        }
-        { right. apply CIH. econs 2; eauto. etransitivity; eauto. }
-      * exploit MemInv.promise; try apply MEMORY; eauto.
-        { apply WF_SRC. }
-        { apply WF_TGT. }
-        { apply MemInv.sem_bot. }
-        s. i. des. apply MemInv.sem_bot_inv in INV2. subst.
-        exploit Memory.promise_future; try apply PROMISE_SRC; eauto.
-        { apply WF_SRC. }
-        i. des.
-        eexists _, _, _, _. splits; eauto.
-        { instantiate (1 := Thread.mk _ _ _ _). econs 1. econs 6; s; eauto.
-          inv WF_TGT. eapply Commit.future_wf; eauto.
-          etransitivity; eauto. inv MEMORY. apply Memory.splits_future. auto.
-        }
-        { right. apply CIH. econs 3. auto. }
-Qed.
+    + (* store *)
+      inv REORDER; inv STATE; inv INSTR. ss.
+      exploit MemInv.confirm_src; try apply MEMORY; eauto.
+      { econs.
+        - rewrite Memory.join_comm, Memory.bot_join. eauto.
+        - memtac.
+      }
+      i. des. apply MemInv.sem_bot_inv in INV. subst.
+      exploit MemInv.write; try apply MEMORY; eauto.
+      { apply WF_SRC. }
+      { apply WF_TGT. }
+      { admit. (* promise bot *) }
+      i. des.
+      exploit Memory.write_future; try apply WRITE_SRC; eauto.
+      { apply WF_SRC. }
+      i. des.
+      exploit Memory.write_get; try apply WRITE_SRC; eauto.
+      { apply WF_SRC. }
+      intro GET_SRC.
+      exploit CommitFacts.write_min_spec; try apply GET_SRC; eauto.
+      { eapply Snapshot.writable_mon; [|apply COMMIT].
+        etransitivity; [|apply COMMIT2]. apply COMMIT1.
+      }
+      { etransitivity; [|apply COMMIT]. admit. (* Snapshot.le *) }
+      { inv WF_SRC. eapply Commit.future_wf; eauto. }
+      { admit. (* wf_snapshot *) }
+      i. des.
+      exploit CommitFacts.write_min_spec; try apply MEMORY_SRC; eauto.
+      { eapply Snapshot.le_on_writable; eauto. apply COMMIT1. }
+      { admit. (* Snapshot.le *) }
+      { admit. (* Commit.wf *) }
+      { admit. (* Memory.get *) }
+      { admit. (* Memory.wf_snapshot *) }
+      i. des.
+      eexists _, _, _, _. splits; try apply SIM2.
+      { econs 2; [|econs 1].
+        econs 1. s. econs 3; s.
+        - econs. econs.
+        - admit. (* Commit.write *)
+        - admit. (* Commit.wf *)
+        - admit. (* Memory.write *)
+      }
+      { econs 1. s. econs 3; s; eauto.
+        - econs. econs.
+        - admit. (* Commit. wf *)
+        - admit. (* Memory.write *)
+      }
+      { right. apply CIH. econs 2.
+        admit. (* Commit.le *)
+      }
+Admitted.
 
 Lemma reorder_sim_stmts
       i1 i2 (REORDER: reorder i1 i2):
